fairis/heap_lang/examples/even_odd/eo_vs_mod2.v
@@ -1,0 +1,447 @@
+From stdpp Require Import decidable.
+From iris.prelude Require Import options.
+From iris.algebra Require Import excl_auth.
+From iris.bi Require Import bi.
+From iris.base_logic.lib Require Import invariants.
+From iris.proofmode Require Import tactics.
+From trillium.prelude Require Export finitary quantifiers sigma classical_instances.
+From trillium.program_logic Require Export weakestpre.
+From trillium.fairness Require Import fairness fair_termination.
+From trillium.fairness.heap_lang Require Export lang lifting tactics proofmode.
+From trillium.fairness.heap_lang Require Import notation.
+From trillium.fairness.heap_lang.examples.even_odd Require Import action_model threads.
+
+
+Import derived_laws_later.bi.
+
+Open Scope nat.
+
+Set Default Proof Using "Type".
+
+Definition start : val :=
+  λ: "l",
+    let: "x" := !"l" in
+    (Fork (incr_loop "l" "x") ;;
+    Fork (incr_loop "l" ("x"+#1))).
+
+
+Section Models.
+  
+  Definition even_AM := thread_model 0. 
+  Definition odd_AM := thread_model 1.
+
+  Definition prodA: Type := PubA + (PrivA + PrivA). 
+  Definition fact_TA (pa: prodA): option (amA even_AM) * option (amA odd_AM) := 
+    match pa with
+    | inl s => (Some $ inl s, Some $ inl s)
+    | inr (inl p) => (Some $ inr p, None)
+    | inr (inr p) => (None, Some $ inr p)
+    end. 
+
+  Definition prod_model := ProdAM (fact_act := fact_TA). 
+
+  Lemma prod_AM_fin_branch': AM_fin_branch' prod_model.
+  Proof. 
+    unshelve eapply prod_AM_fin_branch'.  
+    2, 3: apply thread_AM_fin_branch'. 
+    { exact (fun '(oa1, oa2) => 
+               match oa1, oa2 with
+               | Some (inl pa1), Some _ => inl pa1
+               | Some (inr pa1), None => inr (inl pa1)
+               | None, Some (inr pa2) => inr (inr pa2)
+               | _, _ => inl (step_sync 0)
+               end). }
+    red. intros [?|[?|?]]; reflexivity.
+  Qed. 
+
+  Lemma prod_AM_strong_lr: AM_strong_lr prod_model.
+  Proof. 
+    apply fin_branch_strong.
+    - apply prod_AM_fin_branch'. 
+    - apply prod_AM_step_dec; apply thread_AM_step_dec.
+  Qed.
+
+  Definition the_fair_model: FairModel.
+    unshelve eapply (AM2FM prod_model). 
+  Proof.
+    apply prod_AM_strong_lr. 
+  Defined.
+
+  Definition the_model: LiveModel heap_lang the_fair_model :=
+    {| lm_fl (x: fmstate the_fair_model) := 61%nat; |}.
+
+End Models.  
+
+(** The CMRAs we need. *)
+Class evenoddPreG (Σ: gFunctors) := {
+  threadPre_G :> threadPreG Σ;
+  (* evenodd_PreG :> inG Σ (excl_authR natO); *)
+ }.
+
+Class evenoddG (Σ: gFunctors) := EvenoddG {
+  even_name: gname;
+  odd_name: gname;
+  eoPreG :> evenoddPreG Σ;
+  (* evenodd_n_G :> inG Σ (excl_authR natO); *)
+  (* thread_G :> threadG Σ; *)
+ }.
+
+(* Definition evenoddΣ : gFunctors := *)
+(*   #[ heapΣ the_fair_model; GFunctor (excl_authR natO) ; GFunctor (excl_authR boolO) ]. *)
+
+(* Global Instance subG_evenoddΣ {Σ} : subG evenoddΣ Σ → evenoddPreG Σ. *)
+(* Proof. solve_inG. Qed. *)
+
+Section proof.
+  Context `{!heapGS Σ the_model, !evenoddG Σ}.
+  (* Context `{EM__G: ExecutionModel heap_lang M__G} `{@heapGS Σ _ EM__G, evenoddG Σ}. *)
+  (* Context {ifG: fairnessGS the_model Σ}. *)
+
+  Let Ns := nroot .@ "even_odd".
+
+  Local Instance evenThreadG: threadG Σ := {| th_name := even_name |}. 
+  Local Instance oddThreadG: threadG Σ := {| th_name := odd_name |}. 
+
+  Definition even_at := (@th_at _ evenThreadG). 
+  Definition odd_at := (@th_at _ oddThreadG). 
+
+  Definition auth_even_at := (@auth_th_at _ evenThreadG). 
+  Definition auth_odd_at := (@auth_th_at _ oddThreadG).  
+
+  Lemma even_agree N M :
+    even_at N -∗ auth_even_at M -∗ ⌜ M = N ⌝.
+  Proof. apply th_agree. Qed.
+  Lemma odd_agree N M :
+    odd_at N -∗ auth_odd_at M -∗ ⌜ M = N ⌝.
+  Proof. apply th_agree. Qed.
+
+  Lemma even_update P N M:
+     auth_even_at M ∗ even_at N ==∗ auth_even_at P ∗ even_at P.
+  Proof. apply th_update. Qed.
+  Lemma odd_update P N M:
+     auth_odd_at M ∗ odd_at N ==∗ auth_odd_at P ∗ odd_at P.
+  Proof. apply th_update. Qed.
+
+  Definition evenodd_inv_inner n : iProp Σ :=
+    ∃ N,
+      frag_model_is (N, N) ∗ n ↦ #N ∗
+      if Nat.even N
+      then auth_even_at N ∗ auth_odd_at (N+1)
+      else auth_even_at (N+1) ∗ auth_odd_at N.
+  Definition evenodd_inv n := inv Ns (evenodd_inv_inner n).
+
+
+  (* TODO: move *)
+  Lemma even_succ_negb n: Nat.even (S n) = negb $ Nat.even n.
+  Proof. by rewrite Nat.even_succ Nat.negb_even. Qed.
+
+  (* TODO: move *)
+  Lemma odd_succ_negb n: Nat.odd (S n) = negb $ Nat.odd n.
+  Proof. by rewrite Nat.odd_succ Nat.negb_odd. Qed.
+
+  (* TODO: move *)
+  Lemma even_plus1_negb n: Nat.even (n + 1) = negb $ Nat.even n.
+  Proof. by rewrite Nat.add_1_r even_succ_negb. Qed. 
+
+  (* TODO: move *)
+  Lemma odd_plus1_negb n: Nat.odd (n + 1) = negb $ Nat.odd n.
+  Proof. by rewrite Nat.add_1_r odd_succ_negb. Qed.
+
+  (* Lemma even_go_spec tid n (N: nat) f (Hf: f > 40) ι: *)
+  (*   {{{  eo_vs n ι even_name 0 ∗ *)
+  (*        tid ↦M {[ inl ρT := f ]} ∗ own even_name (◯E N) ∗ *)
+  (*        frag_free_roles_are ∅ *)
+  (*   }}} *)
+  (*     incr_loop #n #N @ tid *)
+  (*   {{{ RET #(); tid ↦M ∅ }}}. *)
+  (* Proof. *)
+  (*   apply eo_go_spec; auto. *)
+
+  (*   (* !!! relies on transparent thread_model *) *)
+  (*   intros k. rewrite Nat.even_add. rewrite Nat.add_1_r.   *)
+  (*   destruct (Nat.even k) eqn:E.  *)
+  (*   - simpl. eapply amfm_role_step with (a := inl (step_sync k)). *)
+  (*     econstructor; eauto. *)
+  (*     + econstructor. by rewrite Nat.even_add E. *)
+  (*     + econstructor. rewrite Nat.add_1_r Nat.odd_succ. by rewrite E. *)
+  (*   - simpl. eapply amfm_role_step with (a := inr (inl ())). *)
+  (*     econstructor; eauto. *)
+  (*     econstructor. rewrite Nat.add_0_r -Nat.negb_even E. done. *)
+  (* Qed.  *)
+
+  (* Lemma odd_go_spec tid n (N: nat) f (Hf: f > 40) ι: *)
+  (*   {{{  eo_vs n ι odd_name 1 ∗ *)
+  (*        tid ↦M {[ inr ρT := f ]} ∗ odd_at N ∗ *)
+  (*        frag_free_roles_are ∅ *)
+  (*   }}} *)
+  (*     incr_loop #n #N @ tid *)
+  (*   {{{ RET #(); tid ↦M ∅ }}}. *)
+  (* Proof. *)
+  (*   apply eo_go_spec; auto. *)
+
+  (*   (* !!! relies on transparent thread_model *) *)
+  (*   intros k. rewrite Nat.add_1_r Nat.even_succ.  *)
+  (*   destruct (Nat.odd k) eqn:O.  *)
+  (*   - simpl. eapply amfm_role_step with (a := inl (step_sync k)). *)
+  (*     econstructor; eauto. *)
+  (*     + econstructor. by rewrite Nat.odd_add O. *)
+  (*     + econstructor. rewrite Nat.add_1_r Nat.even_succ. by rewrite O. *)
+  (*   - simpl. eapply amfm_role_step with (a := inr (inr ())). *)
+  (*     econstructor; eauto. *)
+  (*     econstructor. rewrite Nat.add_1_r odd_succ_negb O. done. *)
+  (* Qed. *)
+
+  (* TODO: move *)
+  Lemma if_sep_comm (b: bool) (P1 Q1 P2 Q2: iProp Σ):
+     (if b then (P1 ∗ Q1) else (P2 ∗ Q2)) ⊣⊢ (if b then P1 else P2) ∗ (if b then Q1 else Q2).
+  Proof. destruct b; set_solver. Qed. 
+
+  Lemma if_arg_comm {A B: Type} (b: bool) (x y: A) (f: A -> B):
+    (if b then f x else f y) = f (if b then x else y).
+  Proof. by destruct b. Qed. 
+
+  Inductive EO' := eoE | eoO.
+  
+  Definition eo_frag (eo: EO') : nat → iProp Σ :=
+    match eo with
+    | eoE => even_at
+    | eoO => odd_at
+    end.
+
+  (* !!! depends on known role of thread_model *)
+  Definition eo_role (eo: EO'): fmrole the_fair_model :=
+    match eo with
+    | eoE => inl ρT
+    | eoO => inr ρT
+    end.
+
+  (* TODO: require it from thread; abstract over state type *)
+  Lemma odd_syncable n (st: amSt odd_AM) (EVEN: Nat.even n):
+    exists st', amTrans odd_AM st (inl (step_sync n), None) st'.
+  Proof. Admitted. 
+  (* TODO: require it from thread; abstract over state type *)
+  Lemma even_syncable n (st: amSt even_AM) (EVEN: Nat.odd n):
+    exists st', amTrans even_AM st (inl (step_sync n), None) st'.
+  Proof. Admitted. 
+
+  (* TODO: overapproximation. *)
+  (* more relaxed condition would require specifying how LR of factor models
+     are related to LR of the product model *)
+  Lemma even_lr_nonincr (st1 st2: amSt even_AM) a ρ
+    (STEP: amTrans even_AM st1 (a, ρ) st2):
+    AM_live_roles (thread_AM_strong 0) st2 ⊆ AM_live_roles (thread_AM_strong 0) st1. 
+  Proof. Admitted. 
+  Lemma odd_lr_nonincr (st1 st2: amSt odd_AM) a ρ
+    (STEP: amTrans odd_AM st1 (a, ρ) st2):
+    AM_live_roles (thread_AM_strong 1) st2 ⊆ AM_live_roles (thread_AM_strong 1) st1. 
+  Proof. Admitted. 
+  
+  Lemma tfm_live_roles' N: 
+    AM_live_roles prod_AM_strong_lr (N, N) =
+     set_map inl (AM_live_roles (thread_AM_strong 0) N) ∪
+     set_map inr (AM_live_roles (thread_AM_strong 1) N).
+  Proof.
+    apply set_eq. intros ρ.
+    rewrite elem_of_union. rewrite !elem_of_map. 
+    setoid_rewrite <- (AM_live_roles_spec prod_AM_strong_lr).
+    setoid_rewrite <- (AM_live_roles_spec (thread_AM_strong 0)).
+    setoid_rewrite <- (AM_live_roles_spec (thread_AM_strong 1)).
+    split.
+    - intros (?&?&STEP). inversion STEP; subst.
+      1, 3: by left; eexists; split; eauto. 
+      all: by right; eexists; split; eauto.
+    - intros [[ρ1 [-> (a1&?&STEP)]]| [ρ2 [-> (a2&?&STEP)]]].
+      + simpl in a1. unfold TA in a1.
+        destruct a1 as [[n]| ].
+        * inversion STEP; subst. rewrite Nat.add_0_r in H3.
+          edestruct (odd_syncable n n) as [st2' STEP2]; eauto.
+          eexists _, (_, _). simpl.          
+          eapply (@pt_sync1 _ _ _ fact_TA); eauto.
+          Unshelve. 2: exact (inl (step_sync n)). done.
+        * do 2 eexists. simpl. econstructor; eauto.
+          Unshelve. 2: exact (inr $ inl p). done.
+      + simpl in a2. unfold TA in a2.
+        destruct a2 as [[n]| ].
+        * inversion STEP; subst. rewrite Nat.add_1_r Nat.even_succ in H3.
+          edestruct (even_syncable n n) as [st1' STEP1]; eauto.
+          eexists _, (_, _). simpl.          
+          eapply (@pt_sync2 _ _ _ fact_TA); eauto.
+          Unshelve. 2: exact (inl (step_sync n)). done.
+        * do 2 eexists. simpl. econstructor; eauto.
+          Unshelve. 2: exact (inr $ inr p). done.
+  Qed.
+
+  Lemma tfm_live_roles N: 
+    live_roles the_fair_model (N, N) =
+     set_map inl (AM_live_roles (thread_AM_strong 0) N) ∪
+     set_map inr (AM_live_roles (thread_AM_strong 1) N).
+  Proof. apply tfm_live_roles'. Qed. 
+
+  Lemma even_spec tid l (N : nat) ρ f (Hf: f > 40) :
+    {{{ evenodd_inv l ∗ tid ↦M {[ inl ρ := f ]} ∗ even_at N ∗
+        frag_free_roles_are ∅ }}}
+      incr_loop #l #N @ tid
+    {{{ RET #(); tid ↦M ∅ }}}.
+  Proof.
+    iIntros (Φ) "(#Hinv & Hf & Heo & FR) Hk".
+    
+    iApply (@eo_go_spec 0 the_fair_model _ _ _ evenThreadG fst inl 
+             with "[$Hf $FR $Heo]"); [lia| simpl; lia | |done].
+    rewrite /eo_vs. iModIntro.
+    iMod (inv_acc with "Hinv") as "[OPEN CLOS]".
+    { apply top_subseteq. }
+    iDestruct "OPEN" as (M) "(>Hmod & >Hn & Hauths)".
+    rewrite if_sep_comm. iDestruct "Hauths" as "[E O]".
+    iModIntro. iExists _. iSplitL "Hmod Hn E".
+    { rewrite /eo_corr. simpl. iFrame.
+      simpl. iFrame. rewrite Nat.add_0_r. destruct (Nat.even M); auto. }
+    simpl. rewrite Nat.add_0_r.
+    destruct (Nat.even M) eqn:E.
+    - iSplitL.
+      2: { rewrite -Nat.negb_even E. by iIntros "%foo". }
+      iIntros "_ %STEP".
+      edestruct (odd_syncable M M) as [st2' STEP2]; eauto.
+      (* TODO: this will be removed after abstracting threads states
+             and requiring them to agree on N *)      
+      assert (st2' = M + 1) by admit. subst st2'. 
+      iExists ((M + 1), (M + 1)). rewrite !bi.sep_assoc. iSplitR.
+      { iPureIntro. repeat split; auto.
+        - econstructor. simpl. econstructor; eauto.
+          Unshelve. 2: exact (inl (step_sync M)). done.
+        - rewrite !tfm_live_roles'.
+          apply union_mono.
+          + apply set_map_mono; [done| ].
+            eapply even_lr_nonincr; eauto.
+          + apply set_map_mono; [done| ].
+            eapply odd_lr_nonincr; eauto. }
+      iIntros "(?&?&?)". iMod ("CLOS" with "[-]") as "_"; [| done].
+      iNext. iFrame. simpl. 
+      rewrite !Nat.add_0_r.
+      rewrite even_plus1_negb E. simpl. iFrame.
+    - iSplitR.
+      { by iIntros "%?". }
+      iIntros "%O" (a) "%STEP1".
+      iExists (M, M). rewrite !bi.sep_assoc. iSplitR.
+      { iPureIntro. repeat split; auto.
+        econstructor. simpl. econstructor; eauto.
+        Unshelve. 2: exact (inr $ inl a). done. }
+      iIntros "(?&?&?)". iMod ("CLOS" with "[-]") as "_"; [| done].
+      iNext. iFrame. simpl. 
+      rewrite !Nat.add_0_r. rewrite E. iFrame.
+  Admitted. 
+  
+  Lemma odd_spec tid l (N : nat) ρ f (Hf: f > 40) :
+    {{{ evenodd_inv l ∗ tid ↦M {[ inr ρ := f ]} ∗ odd_at N ∗
+        frag_free_roles_are ∅ }}}
+      incr_loop #l #N @ tid
+    {{{ RET #(); tid ↦M ∅ }}}.
+  Proof. Admitted. 
+
+  Lemma incr_loop_spec (eo : EO') tid ρ__e ρ__o n (N : nat) f (Hf: f > 40) :
+    {{{ evenodd_inv n ∗ tid ↦M {[ if eo then inl ρ__e else inr ρ__o := f ]} ∗ (eo_frag eo) N ∗
+        frag_free_roles_are ∅ }}}
+      incr_loop #n #N @ tid
+    {{{ RET #(); tid ↦M ∅ }}}.
+  Proof.
+    iIntros (Φ) "(#Hinv & Hf & Heo & FR) Hk".
+    destruct eo; simpl in *. 
+    - iApply (even_spec with "[$Hf $FR $Heo]"); [lia| ..]; done.
+    - iApply (odd_spec with "[$Hf $FR $Heo]"); [lia| ..]; done.
+  Qed. 
+
+End proof.
+
+Section proof_start.
+  Context `{!heapGS Σ the_model, !evenoddG Σ}.
+  Let Ns := nroot .@ "even_odd".
+
+  (* Local Instance evenThreadG: threadG Σ := {| th_name := even_name |}.  *)
+  (* Local Instance oddThreadG: threadG Σ := {| th_name := odd_name |}.  *)
+
+  Lemma frag_free_roles_are_sep: forall fr1 fr2 (DISJ: fr1 ## fr2), 
+        frag_free_roles_are (fr1 ∪ fr2) ⊣⊢ frag_free_roles_are fr1 ∗ frag_free_roles_are fr2.
+  Proof.
+    intros. rewrite /frag_free_roles_are /frag_free_roles_are.    
+    rewrite -gset.gset_op.
+    rewrite -gset.gset_disj_union; auto. 
+    rewrite -own_op. by rewrite -auth_frag_op.
+  Qed. 
+
+  Let ρEven: fmrole the_fair_model := inl ρT.
+  Let ρOdd: fmrole the_fair_model := inr ρT.
+
+  Lemma start_spec tid n N1 N2 f (Hf: f > 60) :
+    {{{ evenodd_inv n ∗ tid ↦M {[ inl ρT := f; inr ρT := f ]} ∗
+        even_at N1 ∗ odd_at N2 ∗ frag_free_roles_are ∅ }}}
+      start #n @ tid
+    {{{ RET #(); tid ↦M ∅ }}}.
+  Proof using All.
+    iIntros (Φ) "(#Hinv & Hf & Heven_at & Hodd_at & HFR) HΦ". unfold start.
+    rewrite <- (union_empty_l_L ∅). 
+    iDestruct (frag_free_roles_are_sep with "HFR") as "[HFR1 HFR2]"; [set_solver| ].
+    wp_pures.
+    wp_bind (Load _).
+    iApply wp_atomic.
+    iInv Ns as (M) "(>Hmod & >Hn & Hauths)" "Hclose".
+    iIntros "!>". wp_load. iIntros "!>".
+    
+    rewrite if_sep_comm !if_arg_comm.
+    iDestruct "Hauths" as "[Heven Hodd]".
+    iDestruct (even_agree with "Heven_at Heven") as %<-.
+    iDestruct (odd_agree with "Hodd_at Hodd") as %<-.
+
+    iAssert ((if Nat.even M then auth_even_at else auth_odd_at) M ∗
+             (if Nat.even M then auth_odd_at else auth_even_at) (M + 1))%I
+      with "[Heven Hodd] "as "[CUR_AUTH NEXT_AUTH]".
+    { destruct (Nat.even M); iFrame. }
+
+    iAssert ((if Nat.even M then even_at else odd_at) M ∗
+             (if Nat.even M then odd_at else even_at) (M + 1))%I
+      with "[Heven_at Hodd_at] "as "[CUR NEXT]".
+    { destruct (Nat.even M); iFrame. }
+
+    iMod ("Hclose" with "[-Hf CUR NEXT HΦ HFR1 HFR2]") as "_".
+    { iIntros "!>". iExists _. iFrame.
+      destruct (Nat.even M); iFrame. }
+    iIntros "!>". wp_pures. wp_bind (Fork _).
+    iApply (wp_role_fork _ tid _ _ _ {[if Nat.even M then ρOdd else ρEven := _]}
+                         {[if Nat.even M then ρEven else ρOdd := _]}
+             with "[Hf ] [CUR HFR1]"). 
+    { apply map_disjoint_dom. rewrite !dom_singleton.
+      destruct (Nat.even M); set_solver. }
+    { intros Hempty%map_positive_l. set_solver. }
+    { rewrite has_fuels_gt_1; last solve_fuel_positive.
+      rewrite !fmap_insert fmap_empty //.      
+      iApply has_fuels_proper; [..| by iFrame]; auto.
+      rewrite !insert_union_singleton_l map_union_empty.
+      destruct (Nat.even M); try reflexivity.
+      f_equiv. rewrite map_union_comm; auto. apply map_disjoint_dom. set_solver. }
+    { iIntros (tid') "!> Hf".
+      iApply (incr_loop_spec (if Nat.even M then eoE else eoO) with "[-]").
+      2: { destruct (Nat.even M); iFrame "#∗". }
+      { lia. }
+      intuition. }
+
+    iIntros "!> Hf".
+    iIntros "!>".
+    wp_pures.
+    iApply (wp_role_fork _ tid _ _ _ ∅ _ with "[Hf] [NEXT HFR2]").
+    { apply map_disjoint_dom. apply map_disjoint_dom. apply map_disjoint_empty_l. }
+    2: { rewrite has_fuels_gt_1; last solve_fuel_positive.
+         rewrite !fmap_insert fmap_empty //.
+         rewrite insert_union_singleton_l. 
+         rewrite map_union_comm; [done|].
+         apply map_disjoint_dom. set_solver. }
+    { rewrite map_empty_union. destruct (Nat.even M); set_solver. }
+    { iIntros (tid') "!> Hf".
+      wp_pures.
+      replace (Z.of_nat M + 1)%Z with (Z.of_nat (M + 1)) by lia.
+      iApply (incr_loop_spec (if Nat.even M then eoO else eoE) with "[-]").
+      2: { destruct (Nat.even M); iFrame "#∗". }
+      { lia. }
+      intuition. }
+
+    iIntros "!> Hf". by iApply "HΦ".
+  Qed.
+
+End proof_start.
